while-program/NTNITypeSoundness.dfy
@@ -1,0 +1,237 @@
+include "WhileProgram.dfy"
+include "NTNITypeSystem.dfy"
+
+module NTNISoundness {
+    import opened WhileProgram
+    import opened NontransitiveFlowType
+
+    /** We prove the nontransitive information flow security is enforced by the type system
+     *  NTNI security for program c:
+     *  For all label l in labels, for all states M1 =CanFlow(l)= M2
+     *  (M1, c) ==>* (M1', Skip) /\ (M2, c) ==>* (M2, Skip)
+     *  we have M1 ={l}= M2
+     *  This says the l component of a state can only be influenced by the components labeled by l'
+     *  with (l', l) in flow as defined by the (global) security policy
+     */
+    
+    // The equivalence relation on states regarding a set of variables
+    predicate Equiv(vctx: VContext, group: BaseType, s1: MState, s2: MState)
+    requires vctx.Keys == s1.Keys == s2.Keys
+    {
+        forall x :: x in vctx.Keys && x in group  ==> s1[x] == s2[x]
+    }
+    // If two states are equivalent to a larger set of variables, then they
+    // must look equivalent to a smaller set of variables
+    lemma EquivalentStates(vctx: VContext, g1: BaseType, g2: BaseType, s1: MState, s2: MState)
+    requires vctx.Keys == s1.Keys == s2.Keys
+    requires g1 <= g2
+    requires Equiv(vctx, g2, s1, s2)
+    ensures Equiv(vctx, g1, s1, s2)
+    {}
+    // Next we have two properties regarding state transitions
+    // First, if none of the updated variables from c is in g1, and s1 -- c --> s2, then s1 =g= s2
+    // lemma LocalUpdate(vctx: VContext, g1: BaseType, HasCmdType(vctx, vpc, c) <= g2, s1: MState, s2: MState, c: Cmd)
+    lemma {:induction false} LocalUpdate(vctx: VContext, vpc: set<Variable>, g1: BaseType, g2: BaseType, s1: MState, s2: MState, n: int, c: Cmd)
+    requires vctx.Keys == s1.Keys == s2.Keys
+    requires validContext(vctx)
+    requires VariablesInCmd(c) <= vctx.Keys 
+    requires vpc <= variables
+    requires HasCmdType(vctx, vpc, c) != Invalid
+    requires GetBaseType(HasCmdType(vctx, vpc, c)) <= g2
+    requires typeOK(s1) && typeOK(s2) && n >= 0
+    requires VariablesInCmd(c) <= s1.Keys == s2.Keys
+    requires Terminates(c, s1, s2, n)
+    requires g1 * g2 == {} // forall v :: v in g2 ==> !(v in g1)
+    ensures Equiv(vctx, g1, s1, s2)
+    decreases n, c
+    {
+        match c {
+            case Skip => // trivial
+            case Assn(x, e) => // assignment
+            case If(e, c1, c2) => // if-then-else
+                var te := HasExprType(vctx, e);
+                var t1 := HasCmdType(vctx, vpc + GetBaseType(te), c1); 
+                var t2 := HasCmdType(vctx, vpc + GetBaseType(te), c2);
+                var s', c' := SmallStepTermination(s1, s2, c, n);
+                if c' == c1 {
+                    assert HasCmdType(vctx, vpc + GetBaseType(HasExprType(vctx, e)), c1) != Invalid;
+                    LocalUpdate(vctx, vpc+ GetBaseType(HasExprType(vctx, e)), g1, g2, s1, s2, n-1, c1);
+                } else {
+                    LocalUpdate(vctx, vpc+ GetBaseType(HasExprType(vctx, e)), g1, g2, s1, s2, n-1, c2);
+                }
+            case  While(e, c1) => // while loop
+                var te := HasExprType(vctx, e);
+                var t1 := HasCmdType(vctx, vpc + GetBaseType(te), c1); 
+                var res := Evaluate(s1, e);
+                if res == 0 {
+                    // trivial
+                } else {
+                    LocalUpdate(vctx, vpc + GetBaseType(HasExprType(vctx, e)), g1, g2, s1, s2, n-1, Seq(c1, c));
+                }
+            case Seq(c1, c2) => // sequential composition
+                var t1, t2 := HasCmdType(vctx, vpc, c1), HasCmdType(vctx, vpc, c2);
+                var s', n' := Sequencing(s1, s2, c1, c2, n);
+                // two sub-cases
+                LocalUpdate(vctx, vpc, g1, g2, s1, s', n', c1);
+                LocalUpdate(vctx, vpc, g1, g2, s', s2, n-n'-1, c2);
+        }
+    }
+    /// An auxiliary lemma for the next lemma
+    lemma EquivEval(vctx: VContext, g: BaseType, s1: MState, s2: MState, e: Expr)
+    requires vctx.Keys == s1.Keys == s2.Keys
+    requires validContext(vctx)
+    requires g <= vctx.Keys // the set of variables in the group must be in the type context
+    requires VariablesInExpr(e) <= vctx.Keys 
+    requires typeOK(s1) && typeOK(s2)
+    requires Equiv(vctx, g, s1, s2)
+    requires GetBaseType(HasExprType(vctx, e)) <= g
+    ensures Evaluate(s1, e) == Evaluate(s2, e)
+    {}
+    // The second property: if x in g and that all variables appearing in e are also in g, then
+    // given s1 =g= s2, s1 -- Assn(x, e) --> s1', and s2 -- Assn(x, e) --> s2'
+    // we must have s1' =g= s2'
+    // lemma StepConsistency()
+    lemma {:induction false} StepConsistency(vctx: VContext, vpc: set<Variable>, g: BaseType, s1: MState, s2: MState, s1': MState, s2': MState,x: Variable, e: Expr)
+    requires vctx.Keys == s1.Keys == s2.Keys == s1'.Keys == s2'.Keys 
+    requires validContext(vctx)
+    requires g <= vctx.Keys // the set of variables in the group must be in the type context
+    requires VariablesInExpr(e) + {x} <= vctx.Keys 
+    requires vpc <= variables
+    requires typeOK(s1) && typeOK(s2) && typeOK(s1') && typeOK(s2')
+    requires vpc <= g // the control context is included in the set of variables in g
+    requires GetBaseType(HasExprType(vctx, e)) <= g // the assigned value is from the set of variables in g
+    requires HasCmdType(vctx, vpc, Assn(x, e)) != Invalid
+    requires TransitionSmallStep(s1, Assn(x, e)) == (s1', Skip)
+    requires TransitionSmallStep(s2, Assn(x, e)) == (s2', Skip)
+    requires Equiv(vctx, g, s1, s2)
+    ensures Equiv(vctx, g, s1', s2')
+    {
+        EquivEval(vctx, g, s1, s2, e);
+        // assert Evaluate(s1, e) == Evaluate(s2, e);
+        assert s1'[x] == s2'[x];
+    }
+    // The following lemmas form the centre of the proof. 
+    function MaxSet(vctx: VContext, vpc: set<Variable>, c:Cmd, vset: set<Variable>): set<Variable>
+    requires vset <= variables 
+    requires validContext(vctx)
+    requires vpc <= variables
+    requires VariablesInCmd(c) <= vctx.Keys 
+    // requires forall x :: x in vctx.Keys ==> vctx[x] <= variables
+    requires forall y :: y in vpc ==> vctx[y] <= vpc
+    requires HasCmdType(vctx, vpc, c) != Invalid
+    {
+        (set v1, v2 | v1 in vset && v2 in vctx[v1] :: v2)
+    }
+    /// The set of Maximal allowed variables are automatically reflexive and transitive
+    /// We also show that this set also complies with the policy defined by CanFlow 
+    /// (this is not provable if not all variables vset are updated in the program execution)
+    lemma MaxSetCanFlow(vctx: VContext, vpc: set<Variable>, c:Cmd, vset: set<Variable>)
+    requires validContext(vctx)
+    requires vset <= variables 
+    requires vpc <= variables
+    requires VariablesInCmd(c) <= vctx.Keys 
+    // requires forall x :: x in vctx.Keys ==> vctx[x] <= variables // already covered by validContext
+    requires forall y :: y in vpc ==> vctx[y] <= vpc // vpc is transitive
+    requires HasCmdType(vctx, vpc, c) != Invalid
+    ensures forall x, y :: x in vctx.Keys && x in MaxSet(vctx, vpc, c, vset * GetBaseType(HasCmdType(vctx, vpc, c))) && y in vctx[x] ==> 
+        (x in vctx[x] && vctx[y] <= vctx[x] <= MaxSet(vctx, vpc, c, vset * GetBaseType(HasCmdType(vctx, vpc, c))))
+    ensures forall x, y :: x in vctx.Keys && x in MaxSet(vctx, vpc, c, vset * GetBaseType(HasCmdType(vctx, vpc, c))) && y in vctx[x] ==> 
+        coarse_label[y] in CanFlow(coarse_label[x])
+    {}
+
+    // // We define for an arbitrary set of variables, MaxSet(vset) is the set of variables that may influcence variables in vset
+    // // We shall then treat MaxSet(vset) as the set of variables of Low level, which should not be influenced by all the other variables
+    lemma {:induction false} MaxSetConsistency(vctx: VContext, 
+                             vpc: set<Variable>, 
+                            vset: set<Variable>, 
+                              s1: MState, s2: MState, s1': MState, s2': MState, 
+                              k1: int, k2: int, c:Cmd)
+    requires vctx.Keys == s1.Keys == s2.Keys == s1'.Keys == s2'.Keys 
+    requires validContext(vctx)
+    requires vset <= vctx.Keys // the set of variables in the group must be in the type context
+    requires vpc <= variables
+    requires typeOK(s1) && typeOK(s2) && typeOK(s1') && typeOK(s2')
+    requires vpc <= vset // the control context is included in the set of variables in vset, need more properties (1,2,3) for vset
+    requires VariablesInCmd(c) <= vctx.Keys 
+    requires HasCmdType(vctx, vpc, c) != Invalid
+    //requires GetBaseType(HasCmdType(vctx, vpc, c)) <= g // the assigned value is from the set of variables in g
+    requires forall x, y :: x in vset && y in vctx[x] ==> vctx[y] <= vctx[x] <= vset
+    requires forall x, y :: x in vset && y in vctx[x] ==> coarse_label[y] in CanFlow(coarse_label[x])
+    requires Equiv(vctx, vset, s1, s2)
+    requires k1 >= 0 && Terminates(c, s1, s1', k1)
+    requires k2 >= 0 && Terminates(c, s2, s2', k2)
+    ensures Equiv(vctx, vset, s1', s2')
+    decreases k1, k2, c
+    {
+        match c {
+            case Skip => // termination
+            case Assn(x, e) => // assignment
+                if x in vset { 
+                    var vpce := GetBaseType(HasExprType(vctx, e));
+                    assert GetBaseType(HasCmdType(vctx, vpc, c)) <= vset;
+                    EquivEval(vctx, vpce, s1, s2, e);
+                    assert Evaluate(s1, e) == Evaluate(s2, e);
+                } else { // LocalUpdate(VContext, set<Variable>, BaseType, BaseType, s1: MState, s2: MState, n: int, c: Cmd)
+                    LocalUpdate(vctx, vpc, vset, {x}, s1, s1', k1, c);
+                    LocalUpdate(vctx, vpc, vset, {x}, s2, s2', k2, c);
+                    assert Equiv(vctx, vset, s1', s2');
+                }
+            case If(e, c1, c2) => // if-then-else
+                var vpce := GetBaseType(HasExprType(vctx, e));
+                if (GetBaseType(HasCmdType(vctx, vpc, c)) * vset) != {}
+                {
+                    var x :| x in (GetBaseType(HasCmdType(vctx, vpc, c)) * vset);
+                    assert vpce <= vctx[x];
+                    assert vpce <= vset; 
+                    assert Equiv(vctx, vpce, s1, s2);
+                    // // EquivEval(vctx: VContext, g: BaseType, s1: MState, s2: MState, e: Expr)
+                    EquivEval(vctx, vpce, s1, s2, e);
+                    assert Evaluate(s1, e) == Evaluate(s2, e);
+                    var res := Evaluate(s1, e);
+                    if res != 0 {
+                        assert k1-1 >= 0 && Terminates(c1, s1, s1', k1-1);
+                        assert k2-1 >= 0 && Terminates(c1, s2, s2', k2-1);
+                        MaxSetConsistency(vctx, vpc + vpce, vset, s1, s2, s1', s2', k1-1, k2-1, c1);
+                    } else {
+                        assert k1-1 >= 0 && Terminates(c2, s1, s1', k1-1);
+                        assert k2-1 >= 0 && Terminates(c2, s2, s2', k2-1);
+                        MaxSetConsistency(vctx, vpc + vpce, vset, s1, s2, s1', s2', k1-1, k2-1, c2);
+                    }
+                } else {
+                    // (GetBaseType(HasCmdType(vctx, vpc, c)) * vset) == {}
+                    var vars := GetBaseType(HasCmdType(vctx, vpc, c));
+                    LocalUpdate(vctx, vpc, vset, vars, s1, s1', k1, c);
+                    LocalUpdate(vctx, vpc, vset, vars, s2, s2', k2, c);
+                    assert Equiv(vctx, vset, s1', s2');
+                }
+            case While(e, c1) => // while-loop
+                var vpce := GetBaseType(HasExprType(vctx, e));
+                if (GetBaseType(HasCmdType(vctx, vpc, c)) * vset) != {}
+                {
+                    var x :| x in (GetBaseType(HasCmdType(vctx, vpc, c)) * vset);
+                    assert vpce <= vctx[x];
+                    assert vpce <= vset; 
+                    assert Equiv(vctx, vpce, s1, s2);
+                    EquivEval(vctx, vpce, s1, s2, e);
+                    assert Evaluate(s1, e) == Evaluate(s2, e);
+                    var res := Evaluate(s1, e);
+                    if res != 0 {
+                        assert k1-1 >= 0 && Terminates(Seq(c1, c), s1, s1', k1-1);
+                        assert k2-1 >= 0 && Terminates(Seq(c1, c), s2, s2', k2-1);
+                        MaxSetConsistency(vctx, vpc + vpce, vset, s1, s2, s1', s2', k1-1, k2-1, Seq(c1, c));
+                    } else {} // trivial
+                } else {
+                    // (GetBaseType(HasCmdType(vctx, vpc, c)) * vset) == {}
+                    var vars := GetBaseType(HasCmdType(vctx, vpc, c));
+                    LocalUpdate(vctx, vpc, vset, vars, s1, s1', k1, c);
+                    LocalUpdate(vctx, vpc, vset, vars, s2, s2', k2, c);
+                    assert Equiv(vctx, vset, s1', s2');
+                }
+            case Seq(c1, c2) => // sequential composition
+                var s12, k12 := Sequencing(s1, s1', c1, c2, k1);
+                var s22, k22 := Sequencing(s2, s2', c1, c2, k2);
+                MaxSetConsistency(vctx, vpc, vset, s1, s2, s12, s22, k12, k22, c1);
+                MaxSetConsistency(vctx, vpc, vset, s12, s22, s1', s2', k1-k12-1, k2-k22-1, c2);
+        }
+    }
+}
